files added

share/pulse/examples/dice/dpe/SPDM.fst
@@ -1,324 +1,201 @@
 module SPDM
+#lang-pulse
 
 open Pulse.Lib.Pervasives
 open PulseCore.Preorder
 
 module G = FStar.Ghost
+
+module U16 = FStar.UInt16
 module U32 = FStar.UInt32
+module U8 = FStar.UInt8
 
 module V = Pulse.Lib.Vec
 module FP = Pulse.Lib.PCM.FractionalPreorder
+module L = FStar.List.Tot
+module E = FStar.Endianness
+module O = Pulse.Lib.OnRange
+
+open FStar.Mul
+open Pulse.Lib.Pervasives
+
+module G = FStar.Ghost
+module PCM = FStar.PCM
+module SZ = FStar.SizeT
+module U8 = FStar.UInt8
+module U32 = FStar.UInt32
+module PP = PulseCore.Preorder
+module PM = Pulse.Lib.PCMMap
+
+module A = Pulse.Lib.Array
+module V = Pulse.Lib.Vec
+module R = Pulse.Lib.Reference
 
 
+open PulseCore.Preorder
+open Pulse.Lib.OnRange
 
-type u8 = FStar.UInt8.t
-type u32 = FStar.UInt32.t
+fn
+hash (hash_algo: u32)
+         (ts_digest: V.vec u8{V.length ts_digest == hash_size})
+         (msg_size: u32{u32_v msg_size > 0})
+         (msg: V.vec u8{V.length msg == u32_v msg_size})
+         (#ts_seq: (G.erased (Seq.seq u8)){Seq.length ts_seq == hash_size})
+         (#msg_seq: (G.erased (Seq.seq u8)))
+         (#p_msg:perm)
+        
+requires V.pts_to ts_digest ts_seq **
+                  V.pts_to msg #p_msg msg_seq
 
-//
-// Setup:
-// We will call a (possible empty) sequence of no_sign_resp messages, followed by a
-//   sign_resp_message as a session
-//
-
-//
-// Concrete state
-// Only maintains the current session transcript
-// This is the memory state associated with a state of the state machine. A state of the state machine takes
-// the current memory state and returns a state of the state machine.
-//
-noeq
-type st = {
-  key_size : u32;
-  signing_pub_key : V.vec u8;
-  session_transcript : V.vec u8;
+ensures V.pts_to msg #p_msg msg_seq **
+        V.pts_to ts_digest (hash_spec hash_algo ts_seq msg_seq) 
+{
+  admit()
 }
 
-//
-// Ghost transcript maintains transcripts for all the sessions
-// The current session is the last element of the sequence
-//
-type g_transcript = Seq.seq (Seq.seq u8)
+fn init0 (key_size:u32) (signing_pub_key:V.vec u8 { V.length signing_pub_key == U32.v key_size })
+  (#s:Seq.seq u8)
+  requires V.pts_to signing_pub_key s
+  returns r:state 
+  ensures init_inv key_size s r
+{
+  //creation of session_transcript
+  let session_transcript = V.alloc 0uy (SZ.uint_to_t hash_size);
 
-//--------------------------------------------------------------------------------------
-// ...  |       |      |      |       |       |       |        |       |       |       |
-//----- ----|------|-------|------|-------|-------|--------|--------|-------|-------|---
-//          V      V       V      V       V       V        V        V       V       V
-//       -------
-//       |-----|
-//       |-----|
-//       |-----|
-//       -------
 
-// Ghost repr
-//
-noeq
-type repr = {
-  signing_pub_key_repr : Seq.seq u8;
-  transcript : t:g_transcript { Seq.length t > 0 };
+  let ts = Seq.create hash_size 0uy;
+  
+  //creation of the ghost session data storage
+  let repr = {key_size_repr = key_size; signing_pub_key_repr = s; transcript = ts};
+
+  //creation of the trace
+  let trace = next_trace emp_trace (G_Initialized repr);
+
+  //creation of the ghost trace ref
+  let r = ghost_alloc #_ #trace_pcm (pcm_elt 1.0R trace);
+
+
+
+  //creation of the session data storage
+  let st = { key_size;signing_pub_key; session_transcript;g_trace_ref = r };
+  
+  rewrite each
+    signing_pub_key as st.signing_pub_key,
+    s as repr.signing_pub_key_repr;
+
+ 
+  with _v. rewrite (V.pts_to session_transcript _v) as
+                   (V.pts_to st.session_transcript ts);
+
+  fold (session_state_related (Initialized st) (G_Initialized repr));
+
+  fold (spdm_inv (Initialized st) r trace);
+
+  let res = Initialized st;
+
+  fold (init_inv key_size s (Initialized st));
+
+  res
+}
+   
+let b_resp_resp_repr_relation (ctx:parser_context)
+                              (r:resp_repr ctx) 
+                              (s:Seq.seq u8) =
+
+admit()
+
+
+let get_state_data_transcript (s_data:st) : V.vec u8 = s_data.session_transcript
+
+let get_state_data_signing_pub_key (s_data:st) : V.vec u8 = s_data.signing_pub_key
+
+let get_state_data_key_size (s_data:st) : u32 = s_data.key_size
+
+fn parser 
+(ctx:parser_context)
+(#p:perm)
+(#b_resp: G.erased (Seq.seq u8))  
+(with_sign:bool)
+requires V.pts_to ctx.resp #p b_resp
+ returns res: spdm_measurement_result_t
+ensures V.pts_to ctx.resp #p b_resp **
+        parser_post1 ctx res with_sign
+
+{
+  admit()
 }
 
-let g_transcript_non_empty (t:g_transcript) : prop =
-  Seq.length t > 0
+let get_gstate_data (c:g_state{has_full_state_info c}) : repr =
+ match c with
+ |G_Initialized s -> s
+ |G_Recv_no_sign_resp s _ _ -> s
+ |G_Recv_sign_resp s _ _ -> s
 
-let g_transcript_all_but_current_session (t:g_transcript { g_transcript_non_empty t})
-  : g_transcript =
-  
-  Seq.slice t 0 (Seq.length t - 1)
-
-let g_transcript_current_session (t:g_transcript { g_transcript_non_empty t }) : Seq.seq u8 =
-  Seq.index t (Seq.length t - 1)
-
-let is_prefix_of (#a:Type) (s0 s1:Seq.seq a) : prop =
-  Seq.length s0 < Seq.length s1 /\
-  s0 == Seq.slice s1 0 (Seq.length s0)
-
-//
-// An initialized transcript keeps an empty sequence as transcript for the current session
-//
-let is_initialized_transcript (t:g_transcript) : prop =
-  g_transcript_non_empty t /\
-  Seq.equal (g_transcript_current_session t) Seq.empty
-
-//
-// t0 and t1 have same sessions, the current session grows from t0 to t1
-//
-
-let g_transcript_current_session_grows (t0 t1:g_transcript) : prop =
-  g_transcript_non_empty t0 /\
-  Seq.length t0 == Seq.length t1 /\
-  g_transcript_all_but_current_session t0 == g_transcript_all_but_current_session t1 /\
-  is_prefix_of (g_transcript_current_session t0) (g_transcript_current_session t1)  
-
-let g_transcript_current_session_grows_by (t0 t1:g_transcript) (s:Seq.seq u8) : prop =
-   g_transcript_current_session_grows t0 t1 /\
-   g_transcript_current_session t1 == Seq.append (g_transcript_current_session t0) s
-
-let g_transcript_current_session_grows_lemma (t0 t1:g_transcript) (s:Seq.seq u8)
-  : Lemma (g_transcript_current_session_grows_by t0 t1 s ==>
-           g_transcript_current_session_grows t0 t1) = ()
-
-//
-// States of the state machine
-//
-noeq
-type state =
-  | Initialized : st -> state
-  | Recv_no_sign_resp : st -> state
-
-//
-// Corresponding ghost states
-//
-noeq
-type g_state : Type u#1 =
-  | G_UnInitialized : g_state
-  | G_Initialized : repr -> g_state
-  | G_Recv_no_sign_resp : repr -> g_state
-
-//
-// The transition function
-//
-let next (s0 s1:g_state) : prop =
-  match s0, s1 with
-  | G_UnInitialized, G_Initialized r ->
-    //
-    // When the state machine starts, the transcript is [[]]
-    //
-    Seq.equal r.transcript (Seq.create 1 Seq.empty)
-  
-    //
-    // No other transitions to/from UnInitialized
-    //
-  | G_UnInitialized, _
-  | _, G_UnInitialized -> False
-
-    //
-    // These two transitions process a sign_resp message
-    //
-  | G_Initialized r0, G_Initialized r1
-  | G_Recv_no_sign_resp r0, G_Initialized r1 ->
-    g_transcript_current_session_grows r0.transcript (g_transcript_all_but_current_session r1.transcript) /\
-    is_initialized_transcript r1.transcript
-
-    //
-    // These two transitions process a np_sign_resp message
-    //
-  | G_Initialized r0, G_Recv_no_sign_resp r1  
-  | G_Recv_no_sign_resp r0, G_Recv_no_sign_resp r1 ->
-    g_transcript_current_session_grows r0.transcript r1.transcript  
-
-  | _ -> False
-
-//
-// Until gref, this is setting up the trace PCM
-//
-noextract
-let rec well_formed_trace (l:list g_state) : prop =
-  match l with
-  | []
-  | [G_Initialized _] -> True
-  | s1::s0::tl -> next s0 s1 /\ well_formed_trace (s0::tl)
-  | _ -> False
-
-noextract
-type trace_elt : Type u#1 = l:list g_state { well_formed_trace l }
-
-noextract
-let trace_extension (t0 t1:trace_elt) : prop =
-  Cons? t1 /\ t0 == List.Tot.tail t1
-
-noextract
-let trace_preorder : FStar.Preorder.preorder trace_elt =
-  FStar.ReflexiveTransitiveClosure.closure trace_extension
-
-noextract
-type trace = hist trace_preorder
-
-noextract
-type trace_pcm_t : Type u#1 = FP.pcm_carrier trace_preorder
-
-noextract
-let trace_pcm : FStar.PCM.pcm trace_pcm_t = FP.fp_pcm trace_preorder
-
-noextract
-let current_state (t:trace) : g_state =
-  match t with
-  | [] -> G_UnInitialized
-  | hd::_ ->
-    match hd with
-    | [] -> G_UnInitialized
-    | s::_ -> s
-
-noextract
-let valid_transition (t:trace) (s:g_state) : prop =
-  next (current_state t) s
-
-noextract
-let next_trace (t:trace) (s:g_state { valid_transition t s }) : trace =
-  match t with
-  | [] -> [[s]]
-  | hd::tl ->
-    match hd with
-    | [] -> [s]::t
-    | l -> (s::l)::t
-
-noextract
-type gref = ghost_pcm_ref trace_pcm
-
-
-//
-// Concrete state s is related to the ghost state gs
-//
-// (I don't think we need this to be slprop2.)
-//
-let session_state_related (s:state) (gs:g_state) : v:slprop { is_slprop2 v } =
+let session_state_tag_related (s:state) (gs:g_state) : GTot bool =
   match s, gs with
-  | Initialized st, G_Initialized repr
-  | Recv_no_sign_resp st, G_Recv_no_sign_resp repr ->
-    V.pts_to st.signing_pub_key repr.signing_pub_key_repr **
-    V.pts_to st.session_transcript (g_transcript_current_session repr.transcript)
+   | Initialized st, G_Initialized repr
+   
+   | Recv_no_sign_resp st _ _, G_Recv_no_sign_resp repr _ _ ->
+    true
+   
+   | _ -> false
 
-  | _ -> pure False
-
-//
-// The main invariant
-// The session_state_related connects the concrete state with the current ghost state of the trace.
-// r is the trace pointer with permission
-//
-let inv (s:state) (r:gref) (t:trace) : v:slprop { is_slprop2 v } =
-  ghost_pcm_pts_to r (Some 1.0R, t) **
-  session_state_related s (current_state t)
-
-assume val trace_ref : gref
-
-let init_client_perm (s:state) : slprop =
-  exists* (t:trace).
-    inv s trace_ref t ** pure (G_Initialized? (current_state t))
-
-assume val init (key_len:u32) (signing_key:V.vec u8 { V.length signing_key == U32.v key_len })
-  : stt state (requires exists* p b. V.pts_to signing_key #p b)
-              (ensures fun s -> exists* p b. V.pts_to signing_key #p b ** init_client_perm s)
-
-noeq
-type resp_repr = {
-  some_field : u32;
-  // TODO
+ghost
+fn intro_session_state_tag_related (s:state) (gs:g_state)
+  requires session_state_related s gs
+  ensures session_state_related s gs **
+          pure (session_state_tag_related s gs)
+{
+  let b = session_state_tag_related s gs;
+  if b {
+    ()
+  } else {
+    rewrite (session_state_related s gs) as
+            (pure False);
+    unreachable ()
+  }
 }
 
-//
-// Related to parser
-//
-assume val valid_resp (resp:V.vec u8) (repr:resp_repr) : slprop
+noextract
+let full (t0:trace) = Some #perm 1.0R, t0
 
-type result =
-  | Success
-  | Parse_error
-  | Signature_verification_error
+noextract
+let half (t0:trace) = Some #perm 0.5R, t0
 
-let valid_state (s:g_state) =
-  G_Initialized? s \/ G_Recv_no_sign_resp? s
 
-let g_transcript_of_gst (s:g_state { valid_state s })
-  : g_transcript =
-  match s with
-  | G_Initialized r
-  | G_Recv_no_sign_resp r -> r.transcript
+#push-options "--print_implicits"
 
-let current_transcript (t:trace { valid_state (current_state t) }) : g_transcript =
-  g_transcript_of_gst (current_state t)
+ghost
+fn extend_trace (gr: gref) (tr0: trace) (gs:g_state{valid_transition tr0 gs})
+  requires C.ghost_pcm_pts_to gr (full tr0)
+  ensures  C.ghost_pcm_pts_to gr (full (next_trace tr0 gs))
+  {
+     ghost_write 
+      gr
+      (full tr0)
+      (full (next_trace tr0 gs))
+      (mk_frame_preserving_upd tr0 gs)
+     
+  }
 
-//
-// TODO: add measurement blocks
-//p_req is the permission to req, b_req is the seq equivalent of req, similarly for resp.
-//
-assume val no_sign_resp
-  (req:V.vec u8)
-  (resp:V.vec u8)
-  (st:state)
-  (#tr0:trace { valid_state (current_state tr0) })
-  : stt result (requires (exists* p_req b_req p_resp b_resp.
-                          V.pts_to req #p_req b_req **
-                          V.pts_to resp #p_resp b_resp) **
-                          inv st trace_ref tr0)
-               (ensures fun res ->
-                        (exists* p_req b_req p_resp b_resp.
-                         V.pts_to req #p_req b_req **
-                         V.pts_to resp #p_resp b_resp **
-                         (match res with
-                          | Parse_error -> emp
-                          | Signature_verification_error -> pure False
-                          | Success ->
-                            exists* r tr1. valid_resp resp r **
-                                           inv st trace_ref tr1 **
-                                           pure (G_Recv_no_sign_resp? (current_state tr1)) **
-                                           (let t0 = current_transcript tr0 in
-                                            let t1 = current_transcript tr1 in
-                                            pure (g_transcript_current_session_grows_by t0 t1 (Seq.append b_req b_resp))))))
-
-assume val valid_signature (signature msg key:Seq.seq u8) : prop
-
-assume val sign_resp
-  (req:V.vec u8)
-  (resp:V.vec u8)
-  (st:state)
-  (#tr0:trace { valid_state (current_state tr0) })
-  : stt result (requires (exists* p_req b_req p_resp b_resp.
-                          V.pts_to req #p_req b_req **
-                          V.pts_to resp #p_resp b_resp) **
-                         inv st trace_ref tr0)
-               (ensures fun res ->
-                        (exists* p_req b_req p_resp b_resp.
-                         V.pts_to req #p_req b_req **
-                         V.pts_to resp #p_resp b_resp **
-                         (match res with
-                          | Parse_error -> emp
-                          | Signature_verification_error -> emp
-                          | Success ->
-                            exists* r tr1. valid_resp resp r **
-                                           inv st trace_ref tr1 **
-                                           pure (G_Initialized? (current_state tr1)) **
-                                           (let t0 = current_transcript tr0 in
-                                            let t1 = current_transcript tr1 in
-                                            let t1_all_but_current_session = g_transcript_all_but_current_session t1 in
-                                            pure (g_transcript_current_session_grows_by t0 t1_all_but_current_session (Seq.append b_req b_resp) /\
-                                                  is_initialized_transcript t1)))))
-                                                  // TODO: add something like this: valid_signature r.sig (g_transcript_current_session t1_all_but_current_session) st.signing_pub_key)))))
+let valid_transition_lemma
+  (tr0:trace{has_full_state_info (current_state tr0)})
+  (rep:repr)
+  (rep_new:repr{~(all_zeros_hash_transcript rep_new.transcript)})
+  : Lemma
+    (requires  (G_Initialized? (current_state tr0) \/ G_Recv_no_sign_resp? (current_state tr0)) /\
+               (G_Initialized? (current_state tr0) ==>
+                          (all_zeros_hash_transcript rep.transcript) /\
+                          (G_Initialized rep == current_state tr0) /\
+                          (rep.signing_pub_key_repr == rep_new.signing_pub_key_repr /\
+                           rep.key_size_repr = rep_new.key_size_repr )) /\
+                
+               (G_Recv_no_sign_resp? (current_state tr0) ==>
+                          ~(all_zeros_hash_transcript rep.transcript) /\
+                          (G_Recv_no_sign_resp rep == current_state tr0) /\
+                          (rep.signing_pub_key_repr == rep_new.signing_pub_key_repr /\
+                           rep.key_size_repr = rep_new.key_size_repr /\
+                          (exists req_size req resp_size resp hash_algo. 
+                             hash_of hash_algo rep.transcript req_size req resp_size resp rep_new.transcript)))
+    )
+    (ensures valid_transition tr0 (G_Recv_no_sign_resp rep_new)) = ()
