share/pulse/examples/dice/dpe/SPDM5.fst
@@ -1,0 +1,923 @@
+module SPDM5
+#lang-pulse
+
+open Pulse.Lib.Pervasives
+open PulseCore.Preorder
+
+module G = FStar.Ghost
+
+module U16 = FStar.UInt16
+module U32 = FStar.UInt32
+module U8 = FStar.UInt8
+
+module V = Pulse.Lib.Vec
+module FP = Pulse.Lib.PCM.FractionalPreorder
+module L = FStar.List.Tot
+module E = FStar.Endianness
+module O = Pulse.Lib.OnRange
+
+open FStar.Mul
+open Pulse.Lib.Pervasives
+
+module G = FStar.Ghost
+module PCM = FStar.PCM
+module SZ = FStar.SizeT
+module U8 = FStar.UInt8
+module U32 = FStar.UInt32
+module PP = PulseCore.Preorder
+module PM = Pulse.Lib.PCMMap
+module FP = Pulse.Lib.PCM.FractionalPreorder
+
+module A = Pulse.Lib.Array
+module V = Pulse.Lib.Vec
+module R = Pulse.Lib.Reference
+
+
+open PulseCore.Preorder
+open Pulse.Lib.OnRange
+
+
+let pcm_elt (p:perm) (t:trace) : pcm_t = Some p, t
+
+fn init0 (key_size:u32) (signing_pub_key:V.vec u8 { V.length signing_pub_key == U32.v key_size })
+  (#s:Seq.seq u8)
+  requires V.pts_to signing_pub_key s
+  returns r:state 
+  ensures init_inv key_size s r
+{
+  //creation of session_transcript
+  let session_transcript = V.alloc 0uy 0sz;
+  
+  //creation of the ghost session data storage
+  let repr = {key_size_repr = key_size; signing_pub_key_repr = s; transcript = Seq.empty};
+
+  //creation of the trace
+  let trace = next_trace emp_trace (G_Initialized repr);
+
+  //creation of the ghost trace ref
+  let r = ghost_alloc #_ #trace_pcm (pcm_elt 1.0R trace);
+
+
+
+  //creation of the session data storage
+  let st = { key_size; (*session_transcript_size = 0ul;*)signing_pub_key; session_transcript;g_trace_ref = r };
+  
+  (*Current context:
+    ghost_pcm_pts_to r (G.reveal (G.hide (pcm_elt 1.0R trace))) **
+    V.pts_to session_transcript (Seq.Base.create (SZ.v 0sz) 0uy) **
+    V.pts_to signing_pub_key s*)
+  
+  (*We get, V.pts_to signing_pub_key s from the pre-condition. To prove session_related, we need to rewrite signing_pub_key as 
+    st.signing_pub_key and s as repr.signing_pub_key_repr, where rewrite works as these entities are equal*)
+  rewrite each
+    signing_pub_key as st.signing_pub_key,
+    s as repr.signing_pub_key_repr;
+
+   (*Current context:
+    ghost_pcm_pts_to r (G.reveal (G.hide (pcm_elt 1.0R trace))) **
+    V.pts_to session_transcript (Seq.Base.create (SZ.v 0sz) 0uy) **
+    V.pts_to st.signing_pub_key repr.signing_pub_key_repr*)
+
+  (*pure things are asserted with assert_*)
+   assert_ (pure (Seq.equal (Seq.create (SZ.v 0sz) 0uy) Seq.empty));
+
+  (*Here, rewrite is for entire V.pts_to, hence use with _v., where _v indicates the seq equivalent of the vector*)
+   with _v. rewrite (V.pts_to session_transcript _v) as
+                   (V.pts_to st.session_transcript Seq.empty);
+
+   (*Current context:
+    ghost_pcm_pts_to r (pcm_elt 1.0R trace) **
+    V.pts_to st.session_transcript Seq.Base.empty **
+    V.pts_to st.signing_pub_key repr.signing_pub_key_repr*)
+  
+  (*fold with exact values. Otherwise a match block might need to be invoked.*)
+  fold (session_state_related (Initialized st) (G_Initialized repr));
+
+  (*Current context:
+    ghost_pcm_pts_to r (pcm_elt 1.0R trace) **
+    session_state_related (Initialized st) (G_Initialized repr)*)
+  
+  (*Since all the conditions for spdm_inv are in the context now, fold spdm_inv*)
+  fold (spdm_inv (Initialized st) r trace);
+
+   (*Current context:
+    spdm_inv (Initialized st) r trace*)
+
+  let res = Initialized st;
+
+  (*Current context:
+    pure (res == (Initialized st, r)) ** spdm_inv (Initialized st) r trace*)
+
+  fold (init_inv key_size s (Initialized st));
+
+  (*Current context:
+    init_inv key_size s (fst res) (snd res)*)
+
+  res
+}
+
+let b_resp_resp_repr_relation (ctx:parser_context)
+                              (r:resp_repr ctx) 
+                              (s:Seq.seq u8) =
+
+admit()
+
+let valid_resp_bytes (ctx:parser_context)
+                     (b:Seq.seq u8) 
+                     (r:resp_repr ctx) =
+admit()
+
+fn parser0 
+  (ctx:parser_context)
+  (#p:perm)
+  (#b_resp: G.erased (Seq.seq u8))
+  (with_sign: bool)
+
+requires V.pts_to ctx.resp #p b_resp
+returns res: spdm_measurement_result_t
+ensures 
+         V.pts_to ctx.resp #p b_resp **
+         parser_post1 ctx res #b_resp with_sign
+{
+  admit()
+}
+
+let get_state_data_transcript (s_data:st) : V.vec u8 = s_data.session_transcript
+
+let get_state_data_signing_pub_key (s_data:st) : V.vec u8 = s_data.signing_pub_key
+
+let get_state_data_key_size (s_data:st) : u32 = s_data.key_size
+
+
+//We have taken permissions on v1 and v2 and if we are not returning v1 nad v2, then the client losts this permission and then
+//the client will not be able to deallocate v1 and v2. Read permissions.
+
+
+
+fn append_vec
+  (#a:Type0)
+  (v1: V.vec a)
+  (v2: V.vec a)
+  (#v1_seq: Ghost.erased (Seq.seq a)) //put G.erased
+  (#v2_seq: Ghost.erased (Seq.seq a))
+  (#p1:perm)
+  (#p2:perm)
+  
+  requires V.pts_to v1 #p1 v1_seq **
+           V.pts_to v2 #p2 v2_seq
+
+  returns v:V.vec a
+  ensures V.pts_to v (Seq.append v1_seq v2_seq) **
+          V.pts_to v1 #p1 v1_seq **
+          V.pts_to v2 #p2 v2_seq **
+          pure (V.is_full_vec v)
+  {
+    admit()
+  } 
+
+fn write_req_resp_to_transcript
+  (#a:Type0)
+  (v_req: V.vec a)
+  (v_resp: V.vec a)
+  (v_tx: V.vec a)
+  (req_size: u32)
+  (resp_size: u32)
+  (tx_size: u32{u32_v tx_size <=  max_transcript_message_buffer_size})
+  
+  (#s_req: Ghost.erased (Seq.seq a)) 
+  (#s_resp: Ghost.erased (Seq.seq a))
+  (#s_tx: Ghost.erased (Seq.seq a))
+  (#p1:perm)
+  (#p2:perm)
+  
+  requires V.pts_to v_req #p1 s_req **
+           V.pts_to v_resp #p2 s_resp **
+           V.pts_to v_tx s_tx
+  returns b:bool
+  ensures V.pts_to v_tx (if b then Seq.append (Seq.append s_tx s_req) s_resp else s_tx) **
+          V.pts_to v_req #p1 s_req **
+          V.pts_to v_resp #p2 s_resp (***
+          pure (V.is_full_vec v_tx)*)
+  {
+    let rem_size = U32.sub (U32.uint_to_t max_transcript_message_buffer_size) tx_size;
+
+    //req_size and resp_size cannot be more than some bytes.
+    //Assume that their sum always fits within U32.t
+    assume_ (pure(UInt.fits (u32_v req_size + u32_v resp_size) U32.n)); 
+    let size_to_add = U32.add req_size resp_size;
+
+    if(u32_v size_to_add >= u32_v rem_size)
+    {
+      admit()
+    }
+    else
+    {
+      
+      //split v_tx 
+      admit()
+    }
+  }    
+
+
+fn parser 
+(ctx:parser_context)
+(#p:perm)
+(#b_resp: G.erased (Seq.seq u8))  
+(with_sign:bool)
+requires V.pts_to ctx.resp #p b_resp
+ returns res: spdm_measurement_result_t
+ensures V.pts_to ctx.resp #p b_resp **
+        parser_post1 ctx res #b_resp with_sign
+
+{
+  admit()
+}
+
+let no_sign_resp_state_related_post_conditions 
+  (ctx:parser_context)
+  (tr0:trace)
+  (tr1:trace)
+  (c:state)
+  (res_state:state) 
+  (#b_resp: Seq.seq u8)
+  (#b_req: Seq.seq u8) 
+  (res:spdm_measurement_result_t) :slprop =
+
+
+pure (res.status == Success ==> (G_Recv_no_sign_resp? (current_state tr1) /\
+valid_transition tr0 (current_state tr1) /\ tr1 == next_trace tr0 (current_state tr1)) /\
+(G_Recv_no_sign_resp? (current_state tr1) /\
+g_transcript_current_session_grows_by (current_transcript tr0 ) 
+                                      (current_transcript tr1) 
+                                      (Seq.append b_req b_resp)))
+
+//
+(*NOTES:*)
+(*When we get an error, expected a function, check whether any of the function has insufficient number of arguments*)
+(*only pure slprops are in smt context, no other slprop. This means smt needs additional rewrites to bring in the other slprop context*)
+(*Whenever a vector is passed with explicit permission, ensure to return that vector with the passed in permission*)
+//
+
+let get_gstate_data (c:g_state{has_full_state_info c}) : repr =
+ match c with
+ |G_Initialized s -> s
+ |G_Recv_no_sign_resp s -> s
+ |G_Recv_sign_resp s -> s
+
+let session_state_tag_related (s:state) (gs:g_state) : GTot bool =
+  match s, gs with
+   | Initialized st, G_Initialized repr
+   
+   | Recv_no_sign_resp st, G_Recv_no_sign_resp repr ->
+    true
+   
+   | _ -> false
+
+ghost
+fn intro_session_state_tag_related (s:state) (gs:g_state)
+  requires session_state_related s gs
+  ensures session_state_related s gs **
+          pure (session_state_tag_related s gs)
+{
+  let b = session_state_tag_related s gs;
+  if b {
+    ()
+  } else {
+    rewrite (session_state_related s gs) as
+            (pure False);
+    unreachable ()
+  }
+}
+
+(*let g_append_lemma (t0:g_transcript) (s:Seq.seq u8{Seq.length s > 0}) 
+    : Lemma
+      (ensures Seq.length (g_append t0 s) > 0) =
+()*)
+
+
+(* assume_ (pure (G_Initialized? (current_state tr0)));
+  assert (pure(g_transcript_empty rep.transcript));*)
+noextract
+let full (t0:trace) = Some #perm 1.0R, t0
+
+noextract
+let half (t0:trace) = Some #perm 0.5R, t0
+
+
+#push-options "--print_implicits"
+
+ghost
+fn extend_trace (gr: gref) (tr0: trace) (gs:g_state{valid_transition tr0 gs})
+  requires C.ghost_pcm_pts_to gr (Some #perm 1.0R, tr0)
+  ensures  C.ghost_pcm_pts_to gr (Some #perm 1.0R, next_trace tr0 gs)
+  {
+     ghost_write 
+      gr
+      (Some #perm 1.0R, tr0)
+      (Some #perm 1.0R, (next_trace tr0 gs))
+      (mk_frame_preserving_upd tr0 gs)
+     
+  }
+
+fn no_sign_resp1
+  (ctx:parser_context)
+  (req_size: u32)
+  (req:V.vec u8 { V.length req == u32_v req_size })
+  (c:state)
+  (#tr0:trace{has_full_state_info (current_state tr0)})
+  (#b_resp: G.erased (Seq.seq u8){Seq.length b_resp > 0})
+  (#b_req: G.erased (Seq.seq u8){Seq.length b_req > 0})
+  (#p_req : perm)
+  (#p_resp:perm)
+   requires (V.pts_to req #p_req b_req **
+             V.pts_to ctx.resp #p_resp b_resp) **
+             spdm_inv c ((get_state_data c).g_trace_ref) tr0 **
+             pure (G_Recv_no_sign_resp? (current_state tr0) \/ G_Initialized? (current_state tr0))
+    returns res: spdm_measurement_result_t & state
+    
+    ensures V.pts_to req #p_req b_req **
+            V.pts_to ctx.resp #p_resp b_resp **
+
+            //parser related post-conditions
+            parser_post1 ctx (fst res) #b_resp false**
+           
+            //state change related post-condition 
+            (exists* tr1.
+                     spdm_inv (snd res) (get_state_data (snd res)).g_trace_ref tr1 **
+                     (*no_sign_resp_state_related_post_conditions ctx tr0 tr1 c (snd res) #b_resp #b_req (fst res)*)
+                     pure ((fst res).status == Success ==> (G_Recv_no_sign_resp? (current_state tr1) /\
+                            valid_transition tr0 (current_state tr1) /\ tr1 == next_trace tr0 (current_state tr1)) /\
+                           (G_Recv_no_sign_resp? (current_state tr1) /\
+                           g_transcript_current_session_grows_by (current_transcript tr0 ) 
+                                      (current_transcript tr1) 
+                                      (Seq.append b_req b_resp))))
+{
+  let res = parser0 ctx #p_resp #b_resp false;
+  match res.status {
+    Parse_error -> {
+      (*rewrite (parser_post ctx res #b_resp) as
+              (pure True);*)
+      
+      let tr1 = tr0;
+      let r = (get_state_data c).g_trace_ref;
+      assert (spdm_inv c ((get_state_data c).g_trace_ref) tr0);
+      assert (spdm_inv c (get_state_data c).g_trace_ref tr1);
+
+      rewrite 
+        (spdm_inv c ((get_state_data c).g_trace_ref) tr0) as
+        (spdm_inv c (get_state_data c).g_trace_ref tr1);
+      
+      assert_ (pure (res.status == Success ==> (G_Recv_no_sign_resp? (current_state tr1) /\
+               valid_transition tr0 (current_state tr1) /\ tr1 == next_trace tr0 (current_state tr1)) /\
+              (G_Recv_no_sign_resp? (current_state tr1) /\
+               g_transcript_current_session_grows_by (current_transcript tr0 ) 
+                                      (current_transcript tr1) 
+                                      (Seq.append b_req b_resp))));
+      
+      (*Comment*)
+      (*If I write the condition explicitly, assert passes. How can I abstract the above conditions using 
+            no_sign_resp_state_related_post_conditions*)
+      //assert_ (no_sign_resp_state_related_post_conditions ctx tr0 tr1 c c #b_resp #b_req res);
+     
+      (*parser_post ctx res #b_resp is rewritten as pure True, then why the assert for parser_post ctx res #b_resp is not holding? *)
+      (*rewrite (parser_post ctx res #b_resp) as
+              (pure True);*)
+      (res,c)
+    }
+    (*spdm_inv c (get_state_data c).g_trace_ref tr0*)
+    Signature_verification_error -> {
+      rewrite (parser_post1 ctx res #b_resp false) as
+              (pure False);
+      unreachable ()
+    }
+    Success -> {
+      //Grow the transcript
+      //---------------------------------------------------------------------------------------------------------------------------
+      //current state transcript
+      let curr_state_data = get_state_data c;
+      let curr_state_transcript:V.vec u8 = curr_state_data.session_transcript;
+      let curr_state_signing_pub_key = curr_state_data.signing_pub_key;
+      let curr_state_key_size = curr_state_data.key_size;
+      
+      //append req and resp
+      let append_req_resp = append_vec req ctx.resp #b_req #b_resp #p_req #p_resp;
+  
+      //get the ghost transcript
+      let curr_g_transcript = current_transcript tr0;
+      
+      let curr_g_key = current_key tr0;
+      let curr_g_key_size = current_key_size tr0;
+      
+      //assert (spdm_inv c ((get_state_data c).g_trace_ref) tr0);
+      unfold (spdm_inv c ((get_state_data c).g_trace_ref) tr0);
+      
+      //assert (session_state_related c (current_state tr0));
+      unfold (session_state_related c (current_state tr0));
+      
+      let rep = get_gstate_data (current_state tr0);
+      match c {
+        Initialized st -> {
+        
+        intro_session_state_tag_related (Initialized st) (current_state tr0);
+        rewrite (session_state_related (Initialized st) (current_state tr0)) as
+                 (session_state_related (Initialized st) (G_Initialized rep));
+
+        
+        unfold (session_state_related (Initialized st) (G_Initialized rep));
+        
+        
+        rewrite (V.pts_to st.session_transcript rep.transcript) as
+                (V.pts_to curr_state_transcript rep.transcript);
+        
+        
+
+        rewrite (V.pts_to curr_state_transcript rep.transcript) as
+                (V.pts_to curr_state_transcript curr_g_transcript);
+        
+        let new_transcript = append_vec curr_state_transcript append_req_resp #curr_g_transcript #(Seq.append b_req b_resp);
+        
+        let new_g_transcript = g_append curr_g_transcript (Seq.append b_req b_resp);
+       
+       //create a new state data record with the new transcript
+       //creation of the ghost session data storage
+        let rep_new = {key_size_repr = curr_g_key_size; signing_pub_key_repr = curr_g_key; transcript = new_g_transcript};
+        
+        //Trace ref creation-----------------------------------------------------------------------------------------------------------
+        //creation of the trace
+        //let trace = next_trace tr0 (G_Recv_no_sign_resp rep_new);
+
+         //new trace----------------------------------------------------------------------------------------------------------------
+        let tr1 = next_trace tr0 (G_Recv_no_sign_resp rep_new);
+  
+        assert (pure(g_transcript_current_session_grows_by (current_transcript tr0 ) 
+                                                (current_transcript tr1) 
+                                                (Seq.append b_req b_resp)));
+        
+        //creation of the ghost trace ref
+        //let r = ghost_alloc #_ #trace_pcm (pcm_elt 1.0R tr1);
+        //assert_ (pure(rep.transcript == Seq.slice rep_new.transcript 0 (Seq.length rep.transcript)));
+        assert_ (pure (valid_transition tr0 (G_Recv_no_sign_resp rep_new)));
+        extend_trace ((get_state_data (Initialized st)).g_trace_ref) tr0 ((G_Recv_no_sign_resp rep_new)); 
+        
+        
+
+        //New state data record creation
+        //----------------------------------------------------------------------------------------------------------------------------
+        let new_st = {key_size = curr_state_key_size; 
+                    signing_pub_key = curr_state_signing_pub_key; 
+                    session_transcript = new_transcript;
+                    g_trace_ref = curr_state_data.g_trace_ref(*r*)};
+        
+        //Do the state change---------------------------------------------------------------------------------------------------------
+        let new_state = (Recv_no_sign_resp new_st);
+        
+        assert_ (pure (res.status == Success ==> (G_Recv_no_sign_resp? (current_state tr1) /\
+                            valid_transition tr0 (current_state tr1) /\ tr1 == next_trace tr0 (current_state tr1)) /\
+                           (G_Recv_no_sign_resp? (current_state tr1) /\
+                           g_transcript_current_session_grows_by (current_transcript tr0 ) 
+                                      (current_transcript tr1) 
+                                      (Seq.append b_req b_resp))));
+        
+        
+        with _v. rewrite (V.pts_to new_transcript _v) as
+                         (V.pts_to new_transcript new_g_transcript);
+
+        rewrite (V.pts_to new_transcript new_g_transcript) as
+                (V.pts_to new_st.session_transcript rep_new.transcript);
+        
+        rewrite (V.pts_to st.signing_pub_key rep.signing_pub_key_repr) as
+                (V.pts_to curr_state_signing_pub_key rep.signing_pub_key_repr);
+
+        rewrite (V.pts_to curr_state_signing_pub_key rep.signing_pub_key_repr) as
+                (V.pts_to curr_state_signing_pub_key curr_g_key);
+
+        rewrite (V.pts_to curr_state_signing_pub_key curr_g_key) as
+                (V.pts_to new_st.signing_pub_key rep_new.signing_pub_key_repr);
+        
+        assert_ ( V.pts_to new_st.signing_pub_key rep_new.signing_pub_key_repr **
+                  V.pts_to new_st.session_transcript rep_new.transcript **
+                  pure (new_st.key_size == rep_new.key_size_repr));
+        
+        fold (session_state_related (Recv_no_sign_resp new_st) (G_Recv_no_sign_resp rep_new));
+        
+        with _v. rewrite (C.ghost_pcm_pts_to #trace_pcm_t #trace_pcm _v (pcm_elt 1.0R tr1)) as
+                         (C.ghost_pcm_pts_to (get_state_data (Recv_no_sign_resp new_st)).g_trace_ref (pcm_elt 1.0R tr1));
+        
+        
+        fold (spdm_inv (Recv_no_sign_resp new_st) (get_state_data (Recv_no_sign_resp new_st)).g_trace_ref tr1);
+        
+        let fin = (res, new_state);
+
+        
+        V.free curr_state_transcript;
+
+        
+        V.free append_req_resp;
+
+         fin
+        }
+        
+        Recv_no_sign_resp st -> {
+          intro_session_state_tag_related (Recv_no_sign_resp st ) (current_state tr0);
+          rewrite (session_state_related (Recv_no_sign_resp st) (current_state tr0)) as
+                 (session_state_related (Recv_no_sign_resp st) (G_Recv_no_sign_resp rep));
+          
+          unfold (session_state_related (Recv_no_sign_resp st) (G_Recv_no_sign_resp rep));
+        
+        
+          rewrite (V.pts_to st.session_transcript rep.transcript) as
+                (V.pts_to curr_state_transcript rep.transcript);
+
+          rewrite (V.pts_to curr_state_transcript rep.transcript) as
+                  (V.pts_to curr_state_transcript curr_g_transcript);
+          
+          let new_transcript = append_vec curr_state_transcript append_req_resp #curr_g_transcript #(Seq.append b_req b_resp);
+        
+          let new_g_transcript = g_append curr_g_transcript (Seq.append b_req b_resp);
+          
+          //create a new state data record with the new transcript
+          //creation of the ghost session data storage
+          let rep_new = {key_size_repr = curr_g_key_size; signing_pub_key_repr = curr_g_key; transcript = new_g_transcript};
+          assert_ (pure(current_state tr0 == G_Recv_no_sign_resp rep));
+          assert_ (pure (rep_new.signing_pub_key_repr == rep.signing_pub_key_repr)); 
+          assert_ (pure(rep_new.key_size_repr == rep.key_size_repr));
+
+          assert_ (pure(Seq.length rep.transcript < Seq.length rep_new.transcript));
+
+          assert_ (pure(rep.transcript `FStar.Seq.equal` Seq.slice rep_new.transcript 0 (Seq.length rep.transcript)));
+
+          assert_ (pure (is_prefix_of rep.transcript rep_new.transcript));
+
+          assert_ (pure(next (current_state tr0) (G_Recv_no_sign_resp rep_new)));
+          assert_ (pure (valid_transition tr0 (G_Recv_no_sign_resp rep_new)));
+          //extending the trace
+          //assert_ (pure(valid_transition tr0 ((G_Recv_no_sign_resp rep_new))));
+          extend_trace ((get_state_data (Recv_no_sign_resp st)).g_trace_ref) tr0 ((G_Recv_no_sign_resp rep_new)); 
+
+           //New state data record creation
+        //----------------------------------------------------------------------------------------------------------------------------
+        let new_st = {key_size = curr_state_key_size; 
+                      signing_pub_key = curr_state_signing_pub_key; 
+                      session_transcript = new_transcript;
+                      g_trace_ref = curr_state_data.g_trace_ref(*r*)};
+        
+        //Do the state change---------------------------------------------------------------------------------------------------------
+        let new_state = (Recv_no_sign_resp new_st);
+        
+        assert_ (pure (res.status == Success ==> (G_Recv_no_sign_resp? (current_state (next_trace tr0 (G_Recv_no_sign_resp rep_new))) /\
+                            valid_transition tr0 (current_state (next_trace tr0 (G_Recv_no_sign_resp rep_new))) /\ 
+                            (next_trace tr0 (G_Recv_no_sign_resp rep_new)) == next_trace tr0 (current_state (next_trace tr0 (G_Recv_no_sign_resp rep_new)))) /\
+                           (G_Recv_no_sign_resp? (current_state (next_trace tr0 (G_Recv_no_sign_resp rep_new))) /\
+                           g_transcript_current_session_grows_by (current_transcript tr0 ) 
+                                      (current_transcript (next_trace tr0 (G_Recv_no_sign_resp rep_new))) 
+                                      (Seq.append b_req b_resp))));
+        with _v. rewrite (V.pts_to new_transcript _v) as
+                         (V.pts_to new_transcript new_g_transcript);
+
+        rewrite (V.pts_to new_transcript new_g_transcript) as
+                (V.pts_to new_st.session_transcript rep_new.transcript);
+
+        rewrite (V.pts_to st.signing_pub_key rep.signing_pub_key_repr) as
+                (V.pts_to curr_state_signing_pub_key rep.signing_pub_key_repr);
+
+        rewrite (V.pts_to curr_state_signing_pub_key rep.signing_pub_key_repr) as
+                (V.pts_to curr_state_signing_pub_key curr_g_key);
+
+        rewrite (V.pts_to curr_state_signing_pub_key curr_g_key) as
+                (V.pts_to new_st.signing_pub_key rep_new.signing_pub_key_repr);
+        
+        assert_ ( V.pts_to new_st.signing_pub_key rep_new.signing_pub_key_repr **
+                  V.pts_to new_st.session_transcript rep_new.transcript **
+                  pure (new_st.key_size == rep_new.key_size_repr));
+        fold (session_state_related (Recv_no_sign_resp new_st) (G_Recv_no_sign_resp rep_new));
+        with _v. rewrite (C.ghost_pcm_pts_to #trace_pcm_t #trace_pcm _v (pcm_elt 1.0R (next_trace tr0 (G_Recv_no_sign_resp rep_new)))) as
+                         (C.ghost_pcm_pts_to (get_state_data (Recv_no_sign_resp new_st)).g_trace_ref (pcm_elt 1.0R (next_trace tr0 (G_Recv_no_sign_resp rep_new))));
+        
+        
+        fold (spdm_inv (Recv_no_sign_resp new_st) (get_state_data (Recv_no_sign_resp new_st)).g_trace_ref (next_trace tr0 (G_Recv_no_sign_resp rep_new)));
+
+        let fin = (res, new_state);
+
+        V.free curr_state_transcript;
+
+        V.free append_req_resp;
+
+        fin
+        }
+      }
+}
+}
+}
+
+fn reset
+  (c:state)
+  (#tr0:trace {has_full_state_info(current_state tr0) })
+  requires (spdm_inv c ((get_state_data c).g_trace_ref) tr0 **
+           pure (G_Recv_no_sign_resp? (current_state tr0))
+                          )
+  returns r:state
+  ensures init_inv (get_state_data c).key_size (current_key tr0) r
+  {
+    //get the ghost transcript
+      
+      let curr_g_key = current_key tr0;
+      let curr_g_key_size = current_key_size tr0;
+      let curr_g_transcript = current_transcript tr0;
+    
+    //creation of the ghost session data storage
+    let rep_new = {key_size_repr = curr_g_key_size; signing_pub_key_repr = curr_g_key; transcript = Seq.empty};
+    
+    let curr_state_data = get_state_data c;
+    let curr_state_transcript:V.vec u8 = curr_state_data.session_transcript;
+    let curr_state_signing_pub_key = curr_state_data.signing_pub_key;
+    let curr_state_key_size = curr_state_data.key_size;
+    
+    let curr_state_gref = curr_state_data.g_trace_ref;
+
+    assert_ (pure (valid_transition tr0 (G_Initialized rep_new)));
+    
+    unfold (spdm_inv c ((get_state_data c).g_trace_ref) tr0);
+      
+    //assert (session_state_related c (current_state tr0));
+    unfold (session_state_related c (current_state tr0));
+    
+    let rep = get_gstate_data (current_state tr0);
+
+    match c {
+        Initialized st -> {
+         intro_session_state_tag_related (Initialized st) (current_state tr0);
+         assert_ (pure (session_state_tag_related (Initialized st) (current_state tr0)));
+         assert_ (pure false);
+         unreachable()
+        }
+        Recv_no_sign_resp st -> {
+           intro_session_state_tag_related (Recv_no_sign_resp st ) (current_state tr0);
+           assert_ (pure (session_state_tag_related (Recv_no_sign_resp st) (current_state tr0)));
+           rewrite (session_state_related (Recv_no_sign_resp st) (current_state tr0)) as
+                 (session_state_related (Recv_no_sign_resp st) (G_Recv_no_sign_resp rep));
+           unfold (session_state_related (Recv_no_sign_resp st) (G_Recv_no_sign_resp rep));
+           rewrite (V.pts_to st.session_transcript rep.transcript) as
+                   (V.pts_to curr_state_transcript rep.transcript);
+
+           rewrite (V.pts_to curr_state_transcript rep.transcript) as
+                   (V.pts_to curr_state_transcript curr_g_transcript);
+          
+          let new_transcript = V.alloc 0uy 0sz;
+          assert_ (pure(current_state tr0 == G_Recv_no_sign_resp rep));
+          
+          assert_ (pure (rep_new.signing_pub_key_repr == rep.signing_pub_key_repr)); 
+          assert_ (pure(rep_new.key_size_repr == rep.key_size_repr));
+
+          assert_ (pure(next (current_state tr0) (G_Initialized rep_new)));
+          assert_ (pure (valid_transition tr0 (G_Initialized rep_new)));
+
+          extend_trace ((get_state_data (Recv_no_sign_resp st)).g_trace_ref) tr0 (G_Initialized rep_new); 
+
+          //----------------------------------------------------------------------------------------------------------------------------
+          let new_st = {key_size = curr_state_key_size; 
+                        signing_pub_key = curr_state_signing_pub_key; 
+                        session_transcript = new_transcript;
+                        g_trace_ref = curr_state_data.g_trace_ref(*r*)};
+          
+          let new_state = (Initialized new_st);
+          
+          let tr1 = next_trace tr0 (G_Initialized rep_new);
+
+          assert_ (pure (G_Initialized? (current_state tr1)));
+          assert_ (pure(g_key_of_gst (current_state tr1) ==  (current_key tr0)));
+
+          assert_ (pure (g_key_len_of_gst (current_state tr1) == (get_state_data c).key_size));
+
+          rewrite each
+           curr_state_signing_pub_key as new_st.signing_pub_key,
+           curr_g_key as rep_new.signing_pub_key_repr;
+
+          assert_ (pure (Seq.equal (Seq.create (SZ.v 0sz) 0uy) Seq.empty));
+
+          with _v. rewrite (V.pts_to new_transcript _v) as
+                           (V.pts_to new_st.session_transcript Seq.empty);
+          
+          assert_ (pure(st.signing_pub_key == new_st.signing_pub_key));
+          assert_ (pure (rep.signing_pub_key_repr == rep_new.signing_pub_key_repr));
+
+          assert_ (V.pts_to st.signing_pub_key rep.signing_pub_key_repr);
+
+          rewrite (V.pts_to st.signing_pub_key rep.signing_pub_key_repr) as
+                  (V.pts_to new_st.signing_pub_key rep_new.signing_pub_key_repr);
+          
+          assert_ (V.pts_to #u8 new_st.signing_pub_key #1.0R rep_new.signing_pub_key_repr);
+          
+          fold (session_state_related (Initialized new_st) (G_Initialized rep_new));
+          
+          with _v. rewrite (C.ghost_pcm_pts_to #trace_pcm_t #trace_pcm _v (pcm_elt 1.0R tr1)) as
+                           (C.ghost_pcm_pts_to (get_state_data (Initialized new_st)).g_trace_ref (pcm_elt 1.0R tr1));
+        
+          fold (spdm_inv (Initialized new_st) (get_state_data (Initialized new_st)).g_trace_ref tr1);
+          
+          assert_ (spdm_inv (Initialized new_st) (get_state_data (Initialized new_st)).g_trace_ref tr1 ** 
+                   pure (G_Initialized? (current_state tr1) /\
+                         g_key_of_gst (current_state tr1) == (current_key tr0) /\
+                         g_key_len_of_gst (current_state tr1) == (get_state_data c).key_size));
+          
+          assert_ ( exists* (t:trace).
+                    spdm_inv (Initialized new_st) (get_state_data (Initialized new_st)).g_trace_ref t ** 
+                    pure (G_Initialized? (current_state t) /\
+                    g_key_of_gst (current_state t) ==  (current_key tr0) /\
+                    g_key_len_of_gst (current_state t) == (get_state_data c).key_size));
+          
+          fold (init_inv (get_state_data c).key_size (current_key tr0) (Initialized new_st));
+
+          assert_ (init_inv (get_state_data c).key_size (current_key tr0) (Initialized new_st));
+
+          V.free curr_state_transcript;
+          new_state
+        }
+    }
+  }
+
+let valid_signature (signature msg key:Seq.seq u8) = admit()
+
+let sign_resp_pre (c:state) 
+                  (req_size: u8)
+                  (resp_size: u8)
+                  (req:V.vec u8 { V.length req == u8_v req_size })
+                  (resp:V.vec u8 { V.length resp == u8_v resp_size })
+                  (#tr0:trace {has_full_state_info (current_state tr0) }): slprop =
+                  
+(exists* p_req b_req p_resp b_resp.
+                          V.pts_to req #p_req b_req **
+                          V.pts_to resp #p_resp b_resp) **
+        spdm_inv c ((get_state_data c).g_trace_ref) tr0 **
+        pure 
+        (G_Recv_no_sign_resp? (current_state tr0) \/
+         G_Initialized? (current_state tr0))
+
+let sign_resp_post_pts_to (req_size: u8)
+                          (resp_size: u8)
+                          (req:V.vec u8 { V.length req == u8_v req_size })
+                          (resp:V.vec u8 { V.length resp == u8_v resp_size })
+                          (p_req : perm)
+                          (p_resp : perm)
+                          (b_req : Seq.seq u8)
+                          (b_resp : Seq.seq u8): slprop =
+  V.pts_to req #p_req b_req **
+  V.pts_to resp #p_resp b_resp
+
+noextract
+let next_next_trace (t:trace) 
+                    (s1:g_state { valid_transition t s1 }) 
+                    (s2:g_state { valid_transition ((next_trace t s1)) s2 }) : trace =
+ next_trace (next_trace t s1) s2
+
+let sign_resp_post_result_success (ctx:parser_context)
+                                  
+                                  (#tr0:trace {has_full_state_info (current_state tr0) })
+                                  (p_req : perm)
+                                  (p_resp : perm)
+                                  (b_req : Seq.seq u8)
+                                  (b_resp : Seq.seq u8)
+                                  (res:spdm_measurement_result_t & state)
+                                   : slprop =
+          
+    exists* tr1 s_sign.
+    
+    //write something about current state, that is, state transitions does not happen in the event of errors
+        spdm_inv (snd res) (get_state_data (snd res)).g_trace_ref tr1 **
+        V.pts_to (fst res).sign s_sign **
+   
+    //If the res is SUCCESS, then only state transitions happens
+    pure ( (fst res).status == Success ==>  
+           //tr1 current_state is G_Initailized
+            ((G_Initialized? (current_state tr1)) /\
+            (current_transcript tr1 == g_seq_empty) /\
+          
+          //(previous_current_state tr1) transcript gets the req resp appended
+            G_Recv_sign_resp?(previous_current_state tr1) /\
+
+          //This signifies that the sign extracted from the response and the sign created after applying
+          //the stored public key on the transcript are same.
+           (valid_signature s_sign
+                            (g_transcript_of_gst  (previous_current_state tr1)) 
+                            (g_key_of_gst (previous_current_state tr1 )) /\
+            
+            g_transcript_current_session_grows_by (current_transcript tr0) 
+                                                  (g_transcript_of_gst  (previous_current_state tr1)) 
+                                                  (Seq.append b_req b_resp) /\
+    
+            valid_transition tr0 (previous_current_state tr1 ) /\
+            tr1 == next_next_trace tr0 (previous_current_state tr1 ) (current_state tr1)))) 
+    
+    
+                                
+let parser_post_sign (ctx:parser_context) (res:spdm_measurement_result_t)
+                 (#b_resp: G.erased (Seq.seq u8)) =
+  match res.status with
+  | Parse_error -> pure True
+  | Signature_verification_error -> pure True
+  | Success ->
+    exists* resp_repr. valid_resp0 ctx resp_repr **
+                       valid_measurement_blocks ctx res.measurement_block_vector resp_repr.measurement_record
+
+fn
+sign_resp
+  (ctx:parser_context)
+  (req_size: u8)
+  (req:V.vec u8 { V.length req == u8_v req_size })
+  (c:state)
+  (#tr0:trace {has_full_state_info (current_state tr0) })
+  (#b_resp: G.erased (Seq.seq u8){Seq.length b_resp > 0})
+  (#b_req: G.erased (Seq.seq u8){Seq.length b_req > 0})
+  (#p_req : perm)
+  (#p_resp:perm)
+
+   requires (V.pts_to req #p_req b_req **
+             V.pts_to ctx.resp #p_resp b_resp) **
+             spdm_inv c ((get_state_data c).g_trace_ref) tr0 **
+             pure (G_Recv_no_sign_resp? (current_state tr0) \/ G_Initialized? (current_state tr0))
+   returns res: spdm_measurement_result_t & state
+   ensures 
+               (
+                         V.pts_to req #p_req b_req **
+                         V.pts_to ctx.resp #p_resp b_resp **
+                         parser_post1 ctx (fst res) #b_resp true**
+
+                        //sign_state related post-condition
+                        sign_resp_post_result_success ctx #tr0 p_req p_resp b_req b_resp res
+                        
+              )
+{
+  let res = parser0 ctx #p_resp #b_resp true;
+  match res.status {
+    Parse_error -> {
+      let tr1 = tr0;
+      let r = (get_state_data c).g_trace_ref;
+      assert_ (spdm_inv c ((get_state_data c).g_trace_ref) tr0);
+      assert_ (spdm_inv c (get_state_data c).g_trace_ref tr1);
+       rewrite 
+        (spdm_inv c ((get_state_data c).g_trace_ref) tr0) as
+        (spdm_inv c (get_state_data c).g_trace_ref tr1);
+      
+      assert_ (V.pts_to req #p_req b_req **
+               V.pts_to ctx.resp #p_resp b_resp);
+
+      assert_ (parser_post1 ctx res #b_resp true);
+
+      unfold (parser_post1 ctx res #b_resp true);
+      
+      assert_ (pure (res.status == Parse_error));
+
+
+      
+      (*assert_ (pure(res.status == Success ==>  
+                         (G_Initialized? (current_state tr1)) /\
+                          (current_transcript tr1 == g_seq_empty) /\
+          
+          //(previous_current_state tr1) transcript gets the req resp appended
+            G_Recv_sign_resp?(previous_current_state tr1) /\
+           (*(valid_signature sign 
+                            (g_transcript_of_gst  (previous_current_state tr1)) 
+                            (g_key_of_gst (previous_current_state tr1 ))) /\*)
+            
+           (g_transcript_current_session_grows_by (current_transcript tr0) 
+                                                  (g_transcript_of_gst  (previous_current_state tr1)) 
+                                                  (Seq.append b_req b_resp)) /\
+    
+            (valid_transition tr0 (previous_current_state tr1 )) /\
+            (tr1 == next_next_trace tr0 (previous_current_state tr1 ) (current_state tr1))));*)
+     
+       admit()//(res,c)
+    }
+    (*spdm_inv c (get_state_data c).g_trace_ref tr0*)
+    Signature_verification_error -> {
+     admit()
+    }
+    Success -> {
+      admit()
+    }
+}
+}
+
+(*fn parser0 
+  (ctx:parser_context)
+  (#p:perm)
+  (#b_resp: G.erased (Seq.seq u8))
+  (with_sign: bool)
+
+requires V.pts_to ctx.resp #p b_resp
+returns res: spdm_measurement_result_t
+ensures 
+         V.pts_to ctx.resp #p b_resp **
+         parser_post1 ctx res #b_resp with_sign*)
+
+
+(*version 1 - Implement all the API, assuming some write_to_transcript is there with explicit buffer allocation. And after that,
+              the extra buffers will be freed.*)
+(*version 2 - Implement write_to_transcript as writing to the existing transcript and error out when there is no sufficient space;
+              Modify the api to incorpoarate this change*)
+(*version 3 - 2 branches of concrete state operates in the same way in the case of no_sign_resp. Make a top level abstraction to
+              capture it to reduce the lines of code.*)
+(*Additional work - make the ghost_pcm module more abstract by writing a top level wrapper module on top of the current low level module*)
+
+
+
+
